{
  "nbformat": 4,
  "nbformat_minor": 0,
  "metadata": {
    "colab": {
      "provenance": []
    },
    "kernelspec": {
      "name": "python3",
      "display_name": "Python 3"
    },
    "language_info": {
      "name": "python"
    }
  },
  "cells": [
    {
      "cell_type": "markdown",
      "source": [
        "## Differential Equations\n",
        "\n",
        "1. Solve the following first-order ordinary differential equations:\n",
        "   - $y'(x)= y$\n",
        "   - $y'(x) = \\frac{1}{2y(x)}$\n",
        "  \n",
        "3. Solve the first-order ordinary differential equations using the method of separation of variables for $x$ and $y=y(x)$:\n",
        "\n",
        "   - $\\frac{dy}{dx} = \\frac{x}{y}$\n",
        "   - $\\frac{dy}{dx} = \\frac{y}{x}$\n",
        "   - $\\frac{dy}{dx} = xy$\n",
        "\n",
        "4. Solve the second-order ordinary differential equations:\n",
        "\n",
        "   * $y''(x) + y'(x) = 0$, with boundary conditions $y(0) = 2$ and $y'(0) = -1$\n",
        "\n",
        "   * $y''(x) - y(x)= 0$, with boundary conditions $y(0) = 2$ and $y'(0) = 0$\n",
        "\n",
        "   * $\\frac{d^2\\,y(x)}{dx^2} = -\\omega^2 y(x)$.\n",
        "\n",
        "5. Check if the function $\\psi(t, x) = A \\cos(\\omega t + kx)$ is a solution of the second-order partial differential equation (the so-called \"wave equation\"), where $v = \\frac{\\omega}{k} = \\frac{2\\pi / T}{2\\pi / \\lambda}$:\n",
        "\n",
        "$$\n",
        "\\frac{\\partial^2 \\psi(t, x)}{\\partial t^2} - v^2 \\frac{\\partial^2 \\psi(t, x)}{\\partial x^2} = 0.\n",
        "$$"
      ],
      "metadata": {
        "id": "NsDlNvkcUI_P"
      }
    },
    {
      "cell_type": "markdown",
      "source": [
        "### Solve the following first-order ordinary differential equations:\n",
        "\n",
        "   - $y'(x)= y$\n",
        "\n",
        "Rewrite the equation:\n",
        "  $$\\frac{dy}{dx}=y,\\quad\\frac{dy}{y}=dx$$\n",
        "\n",
        "Integrate both sides:\n",
        "\n",
        "  $$\\int\\frac{1}{y}dy=\\int1dx,\\quad \\ln|y|=x+C$$\n",
        "\n",
        "Exponentiate both sides:\n",
        "  $$|y|=e^{x+C}=e^C\\cdot e^x$$\n",
        "Replece $e^C$ with a constant and finnaly:\n",
        "\n",
        "###$$y(x)=Ce^x$$\n",
        "\n",
        "\n",
        "---\n",
        "\n"
      ],
      "metadata": {
        "id": "-dlKEIyT6CU2"
      }
    },
    {
      "cell_type": "markdown",
      "source": [
        "-  $y'(x) = \\frac{1}{2y(x)}$\n",
        "\n",
        "Rewrite the equation:\n",
        "$$\\frac{dy}{dx}=\\frac{1}{2y},\\quad 2y\\;dy=1\\;dx$$\n",
        "Integrate doth sides:\n",
        "$$\\int2y\\;dy=\\int\\;1\\;dx,\\quad y^2=x+C$$\n",
        "\n",
        "Finnaly:\n",
        "\n",
        "###$$ y(x)=\\sqrt{x+C}$$\n",
        "\n",
        "\n",
        "\n",
        "---\n",
        "\n"
      ],
      "metadata": {
        "id": "mfa3ysvQAAzy"
      }
    },
    {
      "cell_type": "markdown",
      "source": [
        "###Solve the first-order ordinary differential equations using the method of separation of variables for $x$ and $y=y(x)$:\n",
        "\n",
        "   - $\\frac{dy}{dx} = \\frac{x}{y}$\n",
        "\n",
        "Rewrite the equation:\n",
        "\n",
        "$$\\frac{1}{y}\\;dy=x\\;dx$$\n",
        "\n",
        "Integrate doth sides:\n",
        "\n",
        "$$\\int \\frac{1}{y}\\; dy =\\int x\\; dx,\\quad \\ln|y|=\\frac{x^2}{2}+C$$\n",
        "\n",
        "Exponentiate both sides:\n",
        "\n",
        "$$|y|=e^{\\frac{x^2}{2}+C}=e^C\\cdot\\; e^{\\frac{x^2}{2}}$$\n",
        "\n",
        "Finally:\n",
        "\n",
        "###$$y(x)=C\\cdot e^{\\frac{x^2}{2}}$$\n",
        "\n",
        "\n",
        "---\n",
        "\n",
        "\n",
        "- $\\frac{dy}{dx} = \\frac{y}{x}$\n",
        "\n",
        "Rewrite the equation:\n",
        "\n",
        "$$\\frac{dy}{y}=\\frac{dx}{x}$$\n",
        "\n",
        "Integrate both sides:\n",
        "\n",
        "$$\\int\\frac{1}{y}\\;dy=\\int\\frac{1}{x}\\;dx,\\quad \\ln|y|=\\ln|x|+C$$\n",
        "\n",
        "Exponentiate both sides:\n",
        "\n",
        "$$|y|=e^C|x|$$\n",
        "\n",
        "Finally:\n",
        "\n",
        "###$$y(x)=Cx$$\n",
        "\n",
        "\n",
        "---\n",
        "\n",
        "- $\\frac{dy}{dx} = xy$\n",
        "\n",
        "Rewrite the equation:\n",
        "\n",
        "$$\\frac{dy}{y}=x\\;dx$$\n",
        "\n",
        "Integrate both sides:\n",
        "\n",
        "$$\\int\\frac{1}{y}\\;dy=\\int x\\;dx,\\quad \\ln|y|=\\frac{x^2}{2}+C$$\n",
        "\n",
        "Exponentiate both sides:\n",
        "\n",
        "$$|y|=e^{\\frac{x^2}{2}+C}$$\n",
        "\n",
        "Finally:\n",
        "\n",
        "###$$Ce^{\\frac{x^2}{2}}$$\n",
        "\n",
        "\n",
        "\n",
        "---\n",
        "\n",
        "\n",
        "\n",
        "\n",
        "\n"
      ],
      "metadata": {
        "id": "zPeBFOIdBwV1"
      }
    },
    {
      "cell_type": "markdown",
      "source": [
        "### Solve the second-order ordinary differential equations:\n",
        "\n",
        "   * $y''(x) + y'(x) = 0$, with boundary conditions $y(0) = 2$ and $y'(0) = -1$\n",
        "\n",
        "Let $y'(x)=v(x),\\;then\\;v'(x)=y''(x)\\;\\Rightarrow\\;v'(x)+v(x)=0$\n",
        "\n",
        "Then, first-order linear ordinary differential equation for $v(x)$ will look like:\n",
        "\n",
        "$$\\frac{dv}{dx}=-v\\;\\Rightarrow\\;\\frac{dv}{v}=-dx$$\n",
        "\n",
        "Integrate both sides:\n",
        "\n",
        "$$\\ln|v|=-x+C_1\\;\\Rightarrow\\; v=C_1\\cdot e^{-x} \\\\ y'(x)=C_1e^{-x}$$\n",
        "\n",
        "Integrate again:\n",
        "\n",
        "$$y(x)=-C_1\\cdot e^{-x}+C_2$$\n",
        "\n",
        "for $y(0)=2:\\quad -C_1\\cdot e^0+C_2=2\\;\\Rightarrow\\;-C_1+C_2=2\\;\\Rightarrow\\;C_2=2+C_1$\n",
        "\n",
        "for $y'(0)=-1:\\quad C_1\\cdot e^0=-1\\;\\Rightarrow\\;C_1=-1\\;\\Rightarrow\\;C_2=2+C_1\\;\\Rightarrow\\;C_2=2+(-1)=1$\n",
        "\n",
        "Finally:\n",
        "\n",
        "###$$y(x)=e^{-x}+1$$\n",
        "\n",
        "---\n",
        "\n",
        "\n",
        "\n",
        "   * $y''(x) - y(x)= 0$, with boundary conditions $y(0) = 2$ and $y'(0) = 0$\n",
        "\n",
        "   Substituting r into the equation:\n",
        "\n",
        "   $$r^2-1=0\\;\\Rightarrow\\;r=\\pm1 $$\n",
        "\n",
        "   $y(x)=C_1e^x+C_2e^{-x}$\n",
        "\n",
        "for $y(0)=2: \\\\ C_1e^0+C_2e^0=0\\;\\Rightarrow\\; C_1+C_2=2$\n",
        "\n",
        "for $y'(0)=0: \\\\ C_1e^0-C_2e^0=0\\;\\Rightarrow\\;C_1-C_2=0\\;\\Rightarrow\\; C_1=C_2$\n",
        "\n",
        "then: $$2C_1=2\\;\\Rightarrow\\;C_1=1\\;\\Rightarrow\\;C_2=1$$\n",
        "\n",
        "Finally:\n",
        "\n",
        "###$$e^x+e^{-x}$$\n",
        "\n",
        "\n",
        "  \n",
        "\n",
        "\n",
        "\n",
        "---\n",
        "\n",
        "\n",
        "   \n",
        "\n",
        "   * $\\frac{d^2\\,y(x)}{dx^2} = -\\omega^2 y(x)$.\n",
        "\n",
        "Rewrite the equation:\n",
        "$$y''(x)+\\omega^2y(x)=0$$\n",
        "\n",
        "We could see that $y''(x)$ is a second derivative of $y(x)$ with respec to x.\n",
        "\n",
        "Solve the characteric equation:\n",
        "$$y(x)=e^{rx}$$ substituting this solution into the differential equation:\n",
        "\n",
        "$$\\frac{d^2}{dx^2}e^{rx}=r^2e^{rx}\\;\\Rightarrow\\;r^2e^{rx}+\\omega^2e^{rx}=0|\\div(e^{rx})\\;\\Rightarrow\\; r^2+\\omega^2=0\\;\\Rightarrow\\;r^2=-\\omega^2\\;\\Rightarrow\\;r=\\pm\\sqrt{-\\omega^2}\\;\\Rightarrow\\;r=\\pm i\\omega$$ because $\\sqrt{-1}=i$\n",
        "\n",
        "General solution:\n",
        "\n",
        "\n",
        "\n",
        "\n",
        "---\n",
        "\n",
        "\n"
      ],
      "metadata": {
        "id": "wHn901RJfseR"
      }
    },
    {
      "cell_type": "markdown",
      "source": [
        "###5. Check if the function $\\psi(t, x) = A \\cos(\\omega t + kx)$ is a solution of the second-order partial differential equation (the so-called \"wave equation\"), where $v = \\frac{\\omega}{k} = \\frac{2\\pi / T}{2\\pi / \\lambda}$:\n",
        "\n",
        "$$\n",
        "\\frac{\\partial^2 \\psi(t, x)}{\\partial t^2} - v^2 \\frac{\\partial^2 \\psi(t, x)}{\\partial x^2} = 0.\n",
        "$$\n",
        "\n",
        "1) Compute $\\psi(t,x)=A\\;\\cos(\\omega t+kx)$\n",
        "\n",
        "Differentiate with respect to t:\n",
        "$$\\frac{\\partial\\psi(t,x)}{\\partial t^2}=-A\\omega\\sin(\\omega t+kx)$$\n",
        "\n",
        "Again:\n",
        "$$\\frac{\\partial^2\\psi(t,x)}{\\partial t^2}=-A\\omega^2\\cos(\\omega t+kx)$$\n",
        "\n",
        "Differentiate with respect to x:\n",
        "\n",
        "$$\\frac{\\partial\\psi(t,x)}{\\partial x}=-Ak\\sin(\\omega t+kx)$$\n",
        "\n",
        "Again:\n",
        "\n",
        "$$\\frac{\\partial^2\\psi(t,x)}{\\partial x^2}=-Ak^2\\cos(\\omega t+kx)$$\n",
        "\n",
        "2) Substitute into the wave equation:\n",
        "$$-A\\omega^2\\cos(\\omega t+kx)-v^2(-Ak^2\\cos(\\omega t+kx))=0 \\\\ -A\\cos(\\omega t+kx)(\\omega^2-v^2k^2)=0$$\n",
        "\n",
        "3) Simplify the condition:\n",
        "Since $A\\ne0$ and $\\cos(\\omega t+kx)\\ne0$\n",
        "$$\\omega^2-v^2k^2=0 \\;\\Rightarrow\\; \\omega^2=v^2k^2$$\n",
        "\n",
        "4) Substitute $v$:\n",
        "\n",
        "$$\\frac{\\omega^2}{k^2}\\cdot k^2=\\omega^2\\;\\Rightarrow\\; \\omega^2=\\omega^2$$\n",
        "\n",
        "So the equation is true\n"
      ],
      "metadata": {
        "id": "kCPTumrOsRBJ"
      }
    }
  ]
}